certicoq/theories/L1_5_box/term.v
@@ -36,7 +36,7 @@ Fixpoint print_term (t:Term) : string :=
     | TInd _ => " TIND "
     | TConstruct _ n => " (CSTR " ++ (nat_to_string n) ++ ") "
     | TCase n _ mch _ =>
-      " (CASE " ++ (nat_to_string (fst n)) ++ " _ " ++ (print_term mch) ++
+      " (CASE " ++ (nat_to_string (snd (fst n))) ++ " _ " ++ (print_term mch) ++
                  " _ " ++") "
     | TFix _ n => " (FIX " ++ (nat_to_string n) ++ ") "
   end.
@@ -74,7 +74,7 @@ Proof.
   - destruct t; cross.
     destruct (inductive_dec i i0); destruct (eq_nat_dec n n0); [lft | rght .. ].
   - destruct t2; cross. destruct p as [n l], p0 as [n0 l0].
-    + destruct (eq_nat_dec n n0); destruct (nat_list_dec l l0);
+    + destruct (eq_dec n n0); destruct (nat_list_dec l l0);
       destruct (H t2_1); destruct (H0 t2_2);
       destruct (H1 t2); [lft | rght .. ].
   - destruct t; cross.
